src/succ_graphs.lean
@@ -1,0 +1,40 @@
+import data.pfun
+import logic.relation
+import data.fun_like.basic
+import computability.turing_machine
+
+open relation (refl_trans_gen)
+
+structure execution (σ : Type*) :=
+(next : σ →. option σ)
+(start : σ)
+
+namespace execution
+variables {σ τ : Type*}
+
+def states (f : execution σ) : set σ :=
+{s | refl_trans_gen (λ x y, some y ∈ f.next x) f.start s}
+
+@[elab_as_eliminator]
+theorem induction {P : σ → Prop} (f : execution σ) (base : P f.start)
+  (step : ∀ ⦃x y⦄, P x → some y ∈ f.next x → P y) {x : σ} (hx : x ∈ f.states) : P x :=
+by { induction hx with _ _ _ h ih, { assumption, }, { exact step ih h, } }
+
+
+structure hom (f : execution σ) (g : execution τ) :=
+(to_fun : σ → τ)
+(dom_of : ∀ ⦃x⦄, x ∈ f.states → (g.next (to_fun x)).dom → (f.next x).dom)
+(map_fun : ∀ ⦃x⦄ ⦃y : option σ⦄, x ∈ f.states → y ∈ f.next x → y.map to_fun ∈ g.next (to_fun x))
+(start : to_fun f.start = g.start)
+
+variables (f : execution σ)
+
+def eval : part σ :=
+pfun.fix (λ s, (f.next s).map (λ x, x.elim (sum.inl s) sum.inr)) f.start
+
+-- @[elab_as_eliminator]
+-- theorem eval_induction {P : σ → Prop} {y} (f : execution σ) (hf : y ∈ f.eval)
+--   (base : P y) (step : ∀ ⦃x y'⦄, )
+
+end execution
+
